src/Binary_search_tree.v
@@ -1,0 +1,49 @@
+Require Import Core.
+Require Binary_tree.
+Set Implicit Arguments.
+
+Module Make (S0:SORTABLE) (Extra:ANY).
+  Module S := Sortable_plus S0.
+  Import S.Notations.
+
+  Module BT := Binary_tree.Make S Extra.
+  Include BT.
+  Export  BT.
+
+  Inductive Bounded: A -> A -> T -> Prop :=
+  | singleton_bounded:
+      forall a e,
+        Bounded a a (node a e empty empty)
+  | node_bounded:
+      forall lo1 hi1 t1 lo2 hi2 t2 a e,
+        Bounded lo1 hi1 t1 ->
+        Bounded lo2 hi2 t2 ->
+        hi1 <= a ->
+        a = lo2 ->
+        Bounded lo1 hi2 (node a e t1 t2).
+
+  Inductive Sorted: T -> Prop :=
+  | empty_sorted: Sorted empty
+  | node_sorted:
+      forall lo hi t,
+        Bounded lo hi t -> Sorted t.
+
+
+  Theorem least_is_leftmost:
+    forall (lo hi:A) (t:T),
+      Bounded lo hi t ->
+      Leftmost t lo.
+  Proof
+    fix f lo hi t bnd :=
+    match bnd in Bounded lo hi t
+          return Leftmost t lo with
+    | singleton_bounded a e =>
+      lm_noleft a e empty
+    | @node_bounded
+        lo1 hi1 t1 lo2 hi2 t2 a e
+        bnd1 bnd2 hi1_a a_lo2 =>
+      let p: Leftmost t1 lo1 := f lo1 hi1 t1 bnd1 in
+      @lm_left lo1 a e t1 t2 p
+    end.
+
+End Make.
