src/Binary_tree.v
@@ -1,0 +1,414 @@
+Require Import Core.
+Require Import Coq.Lists.List.
+Import ListNotations.
+Import Equal.Notations.
+
+Set Implicit Arguments.
+
+Module Make (ElementM:ANY) (ExtraM:ANY).
+
+  Definition A := ElementM.T.
+  Definition E := ExtraM.T.
+
+(** * List *)
+(*    ==== *)
+  Module List.
+    Definition L: Set := list A.
+
+    Inductive Permutation: L -> L -> Prop :=
+    | perm_empty:
+        Permutation [] []
+    | perm_prefix:
+        forall x a b, Permutation a b -> Permutation (x::a) (x::b)
+    | perm_swap:
+        forall x y a,  Permutation (x::y::a) (y::x::a)
+    | perm_transitive:
+        forall a b c,  Permutation a b -> Permutation b c -> Permutation a c.
+  End List.
+
+
+
+
+  Inductive T: Set :=
+  | empty: T
+  | node:  A -> E -> T -> T -> T.
+
+  Inductive Height: T -> nat -> Prop :=
+  | empty_height:
+      Height empty 0
+  | node_height:
+      forall t1 h1 t2 h2 a i,
+        Height t1 h1 ->
+        Height t2 h2 ->
+        Height (node a i t1 t2) (1 + max h1 h2).
+
+  Fixpoint height (t:T): nat :=
+    match t with
+    | empty => 0
+    | node _ _ t1 t2 =>
+      1 + max (height t1) (height t2)
+    end.
+
+  Theorem height_is_height:
+    forall t:T, Height t (height t).
+  Proof
+    fix f t :=
+    match t return Height t (height t) with
+    | empty =>
+      empty_height
+    | node a i t1 t2 =>
+      @node_height t1 (height t1) t2 (height t2) a i (f t1) (f t2)
+    end.
+
+  Definition Node (t:T): Prop :=
+    match t with
+    | empty => False
+    | node _ _ _ _ => True
+    end.
+
+  Theorem node_not_empty:
+    forall(a:A) (i:E) (t1 t2: T),
+      node a i t1 t2 <> empty.
+  Proof
+    fun a i t1 t2 p =>
+      Equal.rewrite p Node I.
+
+  Definition is_node (t:T): {Node t} + {~ Node t} :=
+    match t return {Node t} + {~ Node t} with
+      empty => right (fun p:False => match p with end)
+    | node _ _ _ _ => left I
+    end.
+
+  Inductive Element: T -> A -> Prop :=
+  | element_node:
+      forall a e t1 t2, Element (node a e t1 t2) a.
+
+  Inductive Extra: T -> E -> Prop :=
+  | extra_node:
+      forall a e t1 t2, Extra (node a e t1 t2) e.
+
+  Theorem extra_is_node: forall (t:T) (e:E), Extra t e -> Node t.
+  Proof
+    fun t e extra =>
+      match extra in Extra t _ return Node t with
+      | extra_node a e t1 t2 => I
+      end.
+
+  Inductive Leftmost: T -> A -> Prop :=
+  | lm_noleft:
+      forall a e t2, Leftmost (node a e empty t2) a
+  | lm_left:
+      forall x a e t1 t2,
+        Leftmost t1 x ->
+        Leftmost (node a e t1 t2) x.
+
+  Theorem leftmost_is_node:
+    forall (t:T) (a:A),
+      Leftmost t a -> Node t.
+  Proof
+    fix f t a lm :=
+    match lm in Leftmost t a
+          return Node t with
+    | lm_noleft _ _ _ => I
+    | lm_left _ _ _ _ => I
+    end
+  .
+  Fixpoint leftmost (t:T): Node t -> A :=
+    match t return Node t -> A with
+    | empty =>
+      fun nd => match nd with end
+    | node a e t1 t2 =>
+      match is_node t1 with
+      | left  nd => fun _ => leftmost t1 (nd:Node t1)
+      | right p  => fun _ => a
+      end
+    end.
+
+  (* Inorder t xs:  'xs' is the inorder sequence of 't'.*)
+  Section inorder_sequence.
+    Inductive Inorder: T -> list A -> Prop :=
+    | empty_inorder: Inorder empty []
+    | node_inorder:
+        forall t1 xs1 t2 xs2 a e,
+          Inorder t1 xs1 ->
+          Inorder t2 xs2 ->
+          Inorder (node a e t1 t2) (xs1 ++ a :: xs2).
+
+    Fixpoint inorder (t:T): list A :=
+      match t with
+      | empty => []
+      | node a e t1 t2 =>
+        inorder t1 ++ a :: inorder t2
+      end.
+
+    Theorem inorder_correct:
+      forall (t:T) (xs:list A),
+        Inorder t xs ->
+        xs = inorder t.
+    Proof
+      fix f t xs ord :=
+      match ord in Inorder t xs
+            return xs = inorder t with
+      | empty_inorder => eq_refl
+      | @node_inorder t1 xs1 t2 xs2 a e ord1 ord2 =>
+        let eq1: xs1 = inorder t1 := f t1 xs1 ord1 in
+        let eq2: xs2 = inorder t2 := f t2 xs2 ord2 in
+        (equality_chain:
+           (eq_refl: xs1 ++ a :: xs2 = _),
+           (Equal.rewrite eq1 (fun xs => _ = xs ++ a :: xs2) eq_refl
+            : _ = inorder t1 ++ a :: xs2),
+           (Equal.rewrite eq2 (fun xs => _ = inorder t1 ++ a :: xs) eq_refl
+            : _ = inorder t1 ++ a :: inorder t2))
+      end.
+  End inorder_sequence.
+
+
+  (*
+  Theorem leftmost_is_leftmost_new:
+    forall (t:T) (a:A),
+      Leftmost t a ->
+      forall nd:Node t, a = leftmost t nd.
+  Proof
+    fix f t a lm :=
+    match lm in Leftmost t a
+          return forall nd, a = leftmost t nd with
+    | lm_noleft a e t2 =>
+      fun nd => eq_refl
+    | @lm_left x a1 e1 t1 t2 lm1 =>
+      let nd1 := leftmost_is_node lm1 in
+      let eq1: x = leftmost t1 nd1 := f t1 x lm1 nd1 in
+      fun nd =>
+        let f t1_: forall (nd1:Node t1_), x = leftmost (node a e1 t1_ t2) nd :=
+            match t1_ with
+            | empty =>
+              _
+            | node a1 e1 t11 t12 =>
+              _
+            end
+        in
+        _
+    end.
+  *)
+  Theorem leftmost_is_leftmost:
+    forall (t:T) (nd:Node t),
+      Leftmost t (leftmost t nd).
+  Proof
+    let P t nd :=  Leftmost t (leftmost t nd) in
+    fix f t :=
+    match t return forall nd, P t nd with
+    | empty =>
+      fun nd => match nd with end
+    | node a e t1 t2 =>
+      let t_ := node a e t1 t2 in
+      fun nd =>
+        (match
+            t1
+            return (forall nd1, P t1 nd1) -> P (node a e t1 t2) nd
+          with
+          | empty =>
+            let t_ := node a e empty t2 in
+            fun _ =>
+              Equal.rewrite
+                (eq_refl: a = leftmost t_ nd)
+                (fun x => Leftmost t_ a)
+                (lm_noleft a e t2)
+          | node a1 e1 t11 t12 =>
+            let t1_ := node a1 e1 t11 t12 in
+            fun p1: forall nd1, P t1_ nd1 =>
+              let pt1: Leftmost t1_ (leftmost t1_ I) := p1 I in
+              @lm_left (leftmost t1_ I) a e t1_ t2 pt1
+              : Leftmost (node a e t1_ t2) (leftmost (node a e t1_ t2) nd)
+          end) (f t1)
+    end.
+End Make.
+
+
+(*
+Module Make2 (S:SORTABLE).
+  Notation "a <= b"  := (S.Less_equal a b) (at level 70).
+  Notation "a <=? b" := (S.is_less_equal a b) (at level 70).
+  Section sortable.
+    Definition A:Set :=  S.T.
+
+    Theorem transitive: Relation.Transitive S.Less_equal.
+    Proof
+      match S.is_linear_preorder with
+        conj _ tr => tr
+      end.
+
+    Theorem reflexive: Relation.Reflexive S.Less_equal.
+    Proof
+      match S.is_linear_preorder with
+        conj d _ =>
+        Relation.dichotomic_is_reflexive d
+      end.
+
+    Definition Equivalent (a b:A): Prop := a <= b /\ b <= a.
+  End sortable.
+
+
+  Section basic_definitions.
+    Inductive T: Set :=
+    | empty: T
+    | node:  A -> T -> T -> T.
+
+    Inductive Sorted: A -> A -> T -> Prop :=
+    | empty_sorted:
+        forall lo hi: A,
+          lo <= hi ->
+          Sorted lo hi empty
+    | node_sorted:
+        forall lo1 hi1 t1 lo2 hi2 t2 a,
+          Sorted lo1 hi1 t1 ->
+          Sorted lo1 hi2 t2 ->
+          hi1 <= a ->
+          a <= lo2 ->
+          Sorted lo1 hi2 (node a t1 t2).
+
+    Record Guards :=
+      make_guards {low_guard:A; high_guard:A}.
+
+    Definition Sorted_tree (t:T): Prop :=
+      exists g:Guards, Sorted g.(low_guard) g.(high_guard) t.
+  End basic_definitions.
+
+
+  Section inorder_sequence.
+    Fixpoint inorder (t:T): list A :=
+      match t with
+      | empty => [ ]
+      | node a t1 t2 => inorder t1 ++ a :: inorder t2
+      end.
+
+    Definition Same_inorder (t1 t2:T): Prop :=
+      inorder t1 = inorder t2.
+  End inorder_sequence.
+
+
+
+
+  Section find.
+
+    (* A 'Hole' is a partial node where either the left or the right subtree is
+       missing. *)
+    Inductive Hole: Set :=
+    | left_hole:  A -> T -> Hole
+    | right_hole: A -> T -> Hole.
+
+    Definition Path: Set := list Hole.
+
+    Fixpoint tree_of_path (p:list Hole) (t:T): T :=
+      match p with
+      | nil => t
+      | left_hole a r :: holes =>
+        tree_of_path holes (node a t r)
+      | right_hole a l :: holes =>
+        tree_of_path holes (node a l t)
+      end.
+
+
+    Record Focus:Set :=
+      make_focus {
+          path: list Hole;
+          element: A;
+          left: T;
+          right: T}.
+
+    Definition tree_of_focus (f:Focus): T :=
+      tree_of_path f.(path) (node f.(element) f.(left) f.(right)).
+
+    Definition Root_focus (f:Focus) (t:T): Prop :=
+      tree_of_focus f = t /\ f.(path) = [].
+
+    Definition Left_child (f g:Focus): Prop :=
+      f.(path) = left_hole g.(element) g.(right) :: g.(path)
+      /\
+      node f.(element) f.(left) f.(right) = g.(left).
+
+    Definition Right_child (f g:Focus): Prop :=
+      f.(path) = right_hole g.(element) g.(left) :: g.(path)
+      /\
+      node f.(element) f.(left) f.(right) = g.(right).
+
+    Definition Child (f g:Focus): Prop :=
+      Left_child f g \/ Right_child f g.
+
+    Definition focus_root (t:T): {f:Focus | Root_focus f t}
+                                 +
+                                 {t = empty} :=
+      match t with
+      | empty => inright (eq_refl)
+      | node a t1 t2 =>
+        inleft (exist
+                  _
+                  (make_focus [] a t1 t2)
+                  (conj eq_refl eq_refl))
+      end.
+
+    Definition focus_left (f:Focus): {g:Focus| Left_child g f}
+                                     +
+                                     {f.(left) = empty} :=
+      match f with
+      | make_focus path a t1 t2 =>
+        match t1 with
+        | empty => inright eq_refl
+        | node b u1 u2 =>
+          inleft (exist
+                    _
+                    (make_focus
+                       (left_hole a t2 :: path)
+                       b u1 u2)
+                    (conj eq_refl eq_refl))
+        end
+      end.
+
+    Definition focus_right (f:Focus): {g:Focus| Right_child g f}
+                                      +
+                                      {f.(right) = empty} :=
+      match f with
+      | make_focus path a t1 t2 =>
+        match t2 with
+        | empty => inright eq_refl
+        | node b u1 u2 =>
+          inleft (exist
+                    _
+                    (make_focus
+                       (right_hole a t1 :: path)
+                       b u1 u2)
+                    (conj eq_refl eq_refl))
+        end
+      end.
+
+
+
+
+    Inductive Domain: T -> A -> Prop :=
+    | domain_node:
+        forall x a t1 t2,
+          x = a -> Domain (node a t1 t2) x
+    | domain_left:
+        forall x a t1 t2,
+          Domain t1 x -> Domain (node a t1 t2) x
+    | domain_right:
+        forall x a t1 t2,
+          Domain t2 x -> Domain (node a t1 t2) x.
+
+    Definition Found (a:A) (t:T): Set :=
+      {f:Focus | t = tree_of_focus f /\
+                 Equivalent a f.(element)}.
+
+    Definition Not_found (a:A) (t:T): Set :=
+      {p:Path  | t = tree_of_path p empty /\
+                 forall x, Domain t x -> ~ Equivalent a x}.
+
+    Definition Search_result (a:A) (t:T): Set :=
+      Either.T (Found a t) (Not_found a t).
+
+    Definition
+      search (a:A) (t:T): Sorted_tree t -> Search_result a t :=
+      _.
+
+  End find.
+
+
+End Make2.*)
